Propagate core dys changes (#9)
* update flacke.lock to new DY* main

* propagate DY* main changes (trace_length, empty_trace ..)

* moved general functions to DY.Extend

* removing proof fot state pred knowable

dy-extensions/DY.Extend.fst
@@ -5,6 +5,22 @@ open DY.Core
 open DY.Lib
 open DY.Core.Trace.Base
 
+val is_secret_is_knowable: 
+  {|cinvs: crypto_invariants|} ->
+  l:label  -> 
+  tr: trace ->
+  b:bytes ->
+  Lemma 
+  (requires is_secret l tr b)
+  (ensures is_knowable_by l tr b)
+  [SMTPat (is_secret #cinvs l tr b)]
+let is_secret_is_knowable l tr b = ()
+
+let rand_generated_before tr b = 
+  is_not_empty tr /\
+  exists ts. rand_generated_at tr ts b
+
+
 let core_state_was_set_grows  tr1 tr2 prin sid cont:
   Lemma 
   (requires
